Change to Clight in the top-level proof

driver/Compiler.v
@@ -253,12 +253,39 @@ Definition CompCert's_passes :=
   ::: mkpass Asmgenproof.match_prog
   ::: pass_nil _.
 
+
+Definition CLightCompCert's_passes :=
+      mkpass SimplLocalsproof.match_prog
+  ::: mkpass Cshmgenproof.match_prog
+  ::: mkpass Cminorgenproof.match_prog
+  ::: mkpass Selectionproof.match_prog
+  ::: mkpass RTLgenproof.match_prog
+  ::: mkpass (match_if Compopts.optim_tailcalls Tailcallproof.match_prog)
+  ::: mkpass Inliningproof.match_prog
+  ::: mkpass Renumberproof.match_prog
+  ::: mkpass (match_if Compopts.optim_constprop Constpropproof.match_prog)
+  ::: mkpass (match_if Compopts.optim_constprop Renumberproof.match_prog)
+  ::: mkpass (match_if Compopts.optim_CSE CSEproof.match_prog)
+  ::: mkpass (match_if Compopts.optim_redundancy Deadcodeproof.match_prog)
+  ::: mkpass Unusedglobproof.match_prog
+  ::: mkpass Allocproof.match_prog
+  ::: mkpass Tunnelingproof.match_prog
+  ::: mkpass Linearizeproof.match_prog
+  ::: mkpass CleanupLabelsproof.match_prog
+  ::: mkpass (match_if Compopts.debug Debugvarproof.match_prog)
+  ::: mkpass Stackingproof.match_prog
+  ::: mkpass Asmgenproof.match_prog
+  ::: pass_nil _.
+
 (** Composing the [match_prog] relations above, we obtain the relation
   between CompCert C sources and Asm code that characterize CompCert's
   compilation. *)
 
 Definition match_prog: Csyntax.program -> Asm.program -> Prop :=
   pass_match (compose_passes CompCert's_passes).
+
+Definition match_prog_Clight: Clight.program -> Asm.program -> Prop :=
+  pass_match (compose_passes CLightCompCert's_passes).
 
 (** The [transf_c_program] function, when successful, produces
   assembly code that is in the [match_prog] relation with the source C program. *)
@@ -317,6 +344,64 @@ Proof.
   exists tp; split. apply Asmgenproof.transf_program_match; auto.
   reflexivity.
 Qed.
+
+
+(* TODO: this proof by copy-paste is VERY BAD!!!! move it before and use this theorem in the main transf_c_program_match proof *)
+Theorem transf_clight_program_match:
+  forall p tp,
+    transf_clight_program p = OK tp ->
+    match_prog_Clight p tp.
+Proof.
+  intros p1 tp T.
+  (* unfold transf_c_program, time in T. simpl in T. *)
+  (* destruct (SimplExpr.transl_program p) as [p1|e] eqn:P1; simpl in T; try discriminate. *)
+  unfold transf_clight_program, time in T. rewrite ! compose_print_identity in T. simpl in T.
+  destruct (SimplLocals.transf_program p1) as [p2|e] eqn:P2; simpl in T; try discriminate.
+  destruct (Cshmgen.transl_program p2) as [p3|e] eqn:P3; simpl in T; try discriminate.
+  destruct (Cminorgen.transl_program p3) as [p4|e] eqn:P4; simpl in T; try discriminate.
+  unfold transf_cminor_program, time in T. rewrite ! compose_print_identity in T. simpl in T.
+  destruct (Selection.sel_program p4) as [p5|e] eqn:P5; simpl in T; try discriminate.
+  destruct (RTLgen.transl_program p5) as [p6|e] eqn:P6; simpl in T; try discriminate.
+  unfold transf_rtl_program, time in T. rewrite ! compose_print_identity in T. simpl in T.
+  set (p7 := total_if optim_tailcalls Tailcall.transf_program p6) in *.
+  destruct (Inlining.transf_program p7) as [p8|e] eqn:P8; simpl in T; try discriminate.
+  set (p9 := Renumber.transf_program p8) in *.
+  set (p10 := total_if optim_constprop Constprop.transf_program p9) in *.
+  set (p11 := total_if optim_constprop Renumber.transf_program p10) in *.
+  destruct (partial_if optim_CSE CSE.transf_program p11) as [p12|e] eqn:P12; simpl in T; try discriminate.
+  destruct (partial_if optim_redundancy Deadcode.transf_program p12) as [p13|e] eqn:P13; simpl in T; try discriminate.
+  destruct (Unusedglob.transform_program p13) as [p14|e] eqn:P14; simpl in T; try discriminate.
+  destruct (Allocation.transf_program p14) as [p15|e] eqn:P15; simpl in T; try discriminate.
+  set (p16 := Tunneling.tunnel_program p15) in *.
+  destruct (Linearize.transf_program p16) as [p17|e] eqn:P17; simpl in T; try discriminate.
+  set (p18 := CleanupLabels.transf_program p17) in *.
+  destruct (partial_if debug Debugvar.transf_program p18) as [p19|e] eqn:P19; simpl in T; try discriminate.
+  destruct (Stacking.transf_program p19) as [p20|e] eqn:P20; simpl in T; try discriminate.
+  unfold match_prog; simpl.
+  (* exists p1; split. apply SimplExprproof.transf_program_match; auto. *)
+  exists p2; split. apply SimplLocalsproof.match_transf_program; auto.
+  exists p3; split. apply Cshmgenproof.transf_program_match; auto.
+  exists p4; split. apply Cminorgenproof.transf_program_match; auto.
+  exists p5; split. apply Selectionproof.transf_program_match; auto.
+  exists p6; split. apply RTLgenproof.transf_program_match; auto.
+  exists p7; split. apply total_if_match. apply Tailcallproof.transf_program_match.
+  exists p8; split. apply Inliningproof.transf_program_match; auto.
+  exists p9; split. apply Renumberproof.transf_program_match; auto.
+  exists p10; split. apply total_if_match. apply Constpropproof.transf_program_match.
+  exists p11; split. apply total_if_match. apply Renumberproof.transf_program_match.
+  exists p12; split. eapply partial_if_match; eauto. apply CSEproof.transf_program_match.
+  exists p13; split. eapply partial_if_match; eauto. apply Deadcodeproof.transf_program_match.
+  exists p14; split. apply Unusedglobproof.transf_program_match; auto.
+  exists p15; split. apply Allocproof.transf_program_match; auto.
+  exists p16; split. apply Tunnelingproof.transf_program_match.
+  exists p17; split. apply Linearizeproof.transf_program_match; auto.
+  exists p18; split. apply CleanupLabelsproof.transf_program_match; auto.
+  exists p19; split. eapply partial_if_match; eauto. apply Debugvarproof.transf_program_match.
+  exists p20; split. apply Stackingproof.transf_program_match; auto.
+  exists tp; split. apply Asmgenproof.transf_program_match; auto.
+  reflexivity.
+Qed.
+
 
 (** * Semantic preservation *)
 
