security/RSC.v
@@ -4,12 +4,12 @@ Require Import AST Linking Smallstep Events Behaviors.
 Require Import Split.
 
 (* TODO: Change everything to start from Clight instead of C. *)
-Require Import Csyntax Asm.
+Require Import Clight Asm.
 Require Import Compiler Complements.
 
 Section Split.
 
-    Definition c_has_side (s: split) (lr: side) (p: Csyntax.program) :=
+    Definition clight_has_side (s: split) (lr: side) (p: Clight.program) :=
       List.Forall (fun '(id, gd) =>
                      match gd with
                      | Gfun (Ctypes.Internal f) => s (comp_of f) = lr
@@ -25,14 +25,14 @@ Section Split.
                      end)
         (prog_defs p).
 
-    Definition c_compatible (s: split) (p p': Csyntax.program) :=
-      c_has_side s Left p /\ c_has_side s Right p'.
+    Definition clight_compatible (s: split) (p p': Clight.program) :=
+      clight_has_side s Left p /\ clight_has_side s Right p'.
 
     Definition asm_compatible (s: split) (p p': Asm.program) :=
       asm_has_side s Left p /\ asm_has_side s Right p'.
 
     Lemma link_compatible: forall s p p',
-        c_compatible s p p' ->
+        clight_compatible s p p' ->
         Ctypes.prog_pol p = Ctypes.prog_pol p' ->
         exists W, link p p' = Some W.
     Proof.
@@ -46,9 +46,9 @@ Section RSC.
   Variable pol: Policy.t.
   Variable s: split.
 
-  Variable p: Csyntax.program.
+  Variable p: Clight.program.
   Hypothesis pol_p: Ctypes.prog_pol p = pol.
-  Hypothesis p_Left: c_has_side s Left p.
+  Hypothesis p_Left: clight_has_side s Left p.
 
   Variable p_compiled: Asm.program.
 
@@ -58,28 +58,28 @@ Section RSC.
 
   Variable W_t: Asm.program.
 
-  Hypothesis p_p_compiled: transf_c_program p = OK p_compiled.
+  Hypothesis p_p_compiled: transf_clight_program p = OK p_compiled.
   (* TODO: move to Compiler.v file *)
-  Lemma transf_c_program_pol: forall p p',
-      transf_c_program p = OK p' ->
+  Lemma transf_clight_program_pol: forall p p',
+      transf_clight_program p = OK p' ->
       Ctypes.prog_pol p = prog_pol p'.
   Proof.
     admit.
   Admitted.
 
-  Lemma transf_c_program_side: forall p p' lr,
-      transf_c_program p = OK p' ->
-      c_has_side s lr p <-> asm_has_side s lr p'.
+  Lemma transf_clight_program_side: forall p p' lr,
+      transf_clight_program p = OK p' ->
+      clight_has_side s lr p <-> asm_has_side s lr p'.
   Proof.
     admit.
   Admitted.
 
-  Lemma transf_c_program_compatible: forall p1 p1' p2 p2',
-      match_prog p1 p1' ->
-      match_prog p2 p2' ->
+  Lemma transf_clight_program_compatible: forall p1 p1' p2 p2',
+      match_prog_Clight p1 p1' ->
+      match_prog_Clight p2 p2' ->
       (* transf_c_program p1 = OK p1' -> *)
       (* transf_c_program p2 = OK p2' -> *)
-      c_compatible s p1 p2 <-> asm_compatible s p1' p2'.
+      clight_compatible s p1 p2 <-> asm_compatible s p1' p2'.
   Proof.
     admit.
   Admitted.
@@ -94,22 +94,22 @@ Section RSC.
   Admitted.
 
   (* TODO: What does blame mean? *)
-  Axiom c_program_blame: Csyntax.program -> Csyntax.program -> trace -> Prop.
+  Axiom c_program_blame: Clight.program -> Clight.program -> trace -> Prop.
 
-  Axiom backtranslation: Policy.t -> split -> trace -> Csyntax.program * Csyntax.program.
+  Axiom backtranslation: Policy.t -> split -> trace -> Clight.program * Clight.program.
   Axiom backtranslation_correct:
     forall pol s t p C,
       backtranslation pol s t = (p, C) ->
-      c_compatible s p C /\
+      clight_compatible s p C /\
       exists W, link p C = Some W /\
-             c_program_has_initial_trace W t.
+             clight_program_has_initial_trace W t.
 
   Axiom backtranslation_compiles:
     forall pol s t p C,
       backtranslation pol s t = (p, C) ->
       exists p_compiled C_compiled,
-        transf_c_program p = OK p_compiled /\
-          transf_c_program C = OK C_compiled.
+        transf_clight_program p = OK p_compiled /\
+          transf_clight_program C = OK C_compiled.
 
   Axiom backtranslation_pol: forall pol s t,
       Ctypes.prog_pol (fst (backtranslation pol s t)) = pol /\
@@ -117,8 +117,8 @@ Section RSC.
 
   Axiom forward_correctness:
     forall W W' t,
-      match_prog W W' ->
-      c_program_has_initial_trace W t ->
+      match_prog_Clight W W' ->
+      clight_program_has_initial_trace W t ->
       asm_program_has_initial_trace W' t.
 
 
@@ -137,9 +137,10 @@ Section RSC.
   Axiom backward_correctness:
     forall W W' t,
       (* transf_c_program W = OK W' -> *)
-      match_prog W W' ->
+      match_prog_Clight W W' ->
       asm_program_has_initial_trace W' t ->
-      (c_program_has_initial_trace W t \/ exists m, trace_prefix m t /\ m <> t /\ program_behaves (Csem.semantics W) (Goes_wrong m)).
+      (clight_program_has_initial_trace W t \/
+         exists m, trace_prefix m t /\ m <> t /\ program_behaves (Clight.semantics1 W) (Goes_wrong m)).
 
   Definition comp_of_event_or_default (e: event) (cp: compartment) :=
     match e with
@@ -167,20 +168,20 @@ Section RSC.
     forall W W' p1 p2 C t m,
       link p1 C = Some W ->
       link p2 C = Some W' ->
-      c_program_has_initial_trace W' t ->
+      clight_program_has_initial_trace W' t ->
       trace_prefix m t ->
       m <> t ->
-      program_behaves (Csem.semantics W) (Goes_wrong m) ->
+      program_behaves (Clight.semantics1 W) (Goes_wrong m) ->
       blame_on_program m.
 
   Theorem RSC:
     forall (t: trace),
       asm_program_has_initial_trace W_t t ->
-      exists (Cs: Csyntax.program) (W: Csyntax.program),
+      exists (Cs: Clight.program) (W: Clight.program),
         link p Cs = Some W /\
-        (c_program_has_initial_trace W t \/
+        (clight_program_has_initial_trace W t \/
          exists (m: trace), trace_prefix m t /\ m <> t /\
-                         program_behaves (Csem.semantics W) (Goes_wrong m) /\ blame_on_program m).
+                         program_behaves (Clight.semantics1 W) (Goes_wrong m) /\ blame_on_program m).
   Proof.
     intros t H.
     (* Backtranslation *)
@@ -199,9 +200,9 @@ Section RSC.
     (* Forward compiler correctness *)
     pose proof (backtranslation_compiles pol s t p' Cs split_bt) as bt_compiles.
     destruct bt_compiles as [p'_compiled [Cs_compiled [p'_compiles Cs_compiles]]].
-    destruct (@transf_link _ _ _ _ _ (pass_match_link (compose_passes CompCert's_passes))
+    destruct (@transf_link _ _ _ _ _ (pass_match_link (compose_passes CLightCompCert's_passes))
                 p' Cs p'_compiled Cs_compiled Wbt link_bt
-                (transf_c_program_match _ _ p'_compiles) (transf_c_program_match _ _ Cs_compiles)) as [Wbt_compiled [Wbt_compiles ?]].
+                (transf_clight_program_match _ _ p'_compiles) (transf_clight_program_match _ _ Cs_compiles)) as [Wbt_compiled [Wbt_compiles ?]].
     simpl in Wbt_compiled.
     assert (W_compiled_t: asm_program_has_initial_trace Wbt_compiled t).
     { eapply forward_correctness; eauto. }
@@ -209,17 +210,17 @@ Section RSC.
     (* Recomposition *)
     pose proof (recomposition W_t Wbt_compiled) as recomp.
     exploit recomp; eauto.
-    { split; [eapply transf_c_program_side; eauto | eauto]. }
-    { split; [eapply transf_c_program_side; eauto | eapply transf_c_program_side; eauto].
+    { split; [eapply transf_clight_program_side; eauto | eauto]. }
+    { split; [eapply transf_clight_program_side; eauto | eapply transf_clight_program_side; eauto].
     now destruct bt_compat. now destruct bt_compat. }
     clear recomp.
     intros [W' [link_W' W'_t]].
 
     (* Backward compiler correctness *)
-    assert (W_W': match_prog W W').
-    { destruct (@transf_link _ _ _ _ _ (pass_match_link (compose_passes CompCert's_passes))
+    assert (W_W': match_prog_Clight W W').
+    { destruct (@transf_link _ _ _ _ _ (pass_match_link (compose_passes CLightCompCert's_passes))
                 p Cs p_compiled Cs_compiled W link_p_Cs
-                (transf_c_program_match _ _ p_p_compiled) (transf_c_program_match _ _ Cs_compiles)) as [W'' [R G]].
+                (transf_clight_program_match _ _ p_p_compiled) (transf_clight_program_match _ _ Cs_compiles)) as [W'' [R G]].
       assert (W'' = W') by now simpl in *; congruence. subst W''.
       eauto. }
     exploit backward_correctness; eauto.
